

- Let G be the group of reals under addition and G' the group of non-zero reals under multiplication.
Define $\phi : G \rightarrow G'$ s.t.
 $\phi(x) = 2^x$
 $\phi(x + y) = 2^{x+y} = 2^x \cdot 2^y$
- $\phi : \mathbb{Z} \rightarrow \mathbb{Z}_3$
 $\phi(x) = x \pmod{3}$
 $\phi(x + y) = (x + y) \pmod{3}$
 $= (x \pmod{3} + y \pmod{3}) \pmod{3}$
- $\phi : G \rightarrow G/N$, N is a normal subgroup of G .
 $\phi(x) = Nx$
 $\phi(x * y) = N_{x*y} = N_x N_y = \phi(x)\phi(y)$

Defⁿ: Let $\phi : G \rightarrow G'$ be a group homomorphism and let $\text{Ker } \phi = \{x \in G : \phi(x) = e'\}$, where e' is the identity of G' . Call $\text{Ker } \phi$ as the **KERNEL** of ϕ .

Theorem: Let $\phi : G \rightarrow G'$ be a homomorphism, then

- $\phi(e) = e'$
- For every $x \in G$, $\phi(x^{-1}) = [\phi(x)]^{-1}$

Proof:

- $\phi(e) = \phi(ee) = \phi(e)\phi(e)$
 $\phi(e) = e'\phi(e) \rightarrow e'$ is the identity in G'
 $\phi(e)\phi(e) = e'\phi(e)$
 $\Rightarrow \phi(e) = e'$ (by right cancellation)
- $\phi(xx^{-1}) = \phi(x)\phi(x^{-1}) = (1)$
 $= \phi(e) = e' = \phi(x)[\phi(x)]^{-1} = (2)$
 $\phi(x)\phi(x^{-1}) = \phi(x)[\phi(x)]^{-1}$
By left cancellation
 $\phi(x^{-1}) = [\phi(x)]^{-1}$

Theorem: Let $\phi : G \rightarrow G'$ be a homomorphism. $\text{Ker } \phi$ is a normal subgroup of G .

Proof: Let $x, y \in \text{Ker } \phi$, hence $\phi(x) = \phi(y) = e'$.

$$\phi(xy) = \phi(x)\phi(y) = e'e' = e'$$

$$\Rightarrow xy \in \text{Ker } \phi$$

Let $x \in \text{Ker } \phi$, hence $\phi(x) = e'$.

$$\text{Now, } \phi(x^{-1}) = [\phi(x)]^{-1} = [e']^{-1} = e'$$

$$\Rightarrow x^{-1} \in \text{Ker } \phi$$

Thus $\text{Ker } \phi$ is a subgroup of G .

To show that $\text{Ker } \phi$ is a normal subgroup, we need to show that for every $g \in G$ and every $k \in \text{Ker } \phi$, $gkg^{-1} \in \text{Ker } \phi$.

$$\phi(gkg^{-1}) = \phi(g)\phi(k)\phi(g^{-1})$$

$$= \phi(g)\phi(k)\phi(g^{-1})$$

$$= \phi(g)e'\phi(g^{-1})$$

$$= \phi(g)\phi(g^{-1})$$

$$= \phi(g)[\phi(g)]^{-1}$$

$$= e'$$

Hence $gkg^{-1} \in \text{Ker } \phi$ for every $g \in G$ and every $k \in \text{Ker } \phi$.

Let $g' \in G'$, we say that $g \in G$ is an **inverse image** of g' if $\phi(g) = g'$.

Theorem: Let $\phi : G \rightarrow G'$ be a homomorphism with kernel K . For $g' \in G'$, the set of all inverse images of g' is given by the set Kx where x is any particular inverse image of g' .

Proof: Let $g' \in G'$ and $x \in G$ be such that $\phi(x) = g'$.

Now, for any $k \in K$, let $y = kx$.

$$\phi(kx) = \phi(k)\phi(x) = e'\phi(x) = g'$$